lean/privacy/spendability.lean
@@ -1,12 +1,12 @@
 import privacy.actions
 import privacy.amounts
-import privacy.notes.canceled_notes
+import privacy.notes.used_notes
 import privacy.notes.discoverable
 import privacy.utils
 import privacy.transactions.immutability
 
 def spend_note (crypto: Crypto) (m: Memory) (addrbob: ℕ) (kbob: crypto.PrivateKeys) (sn: ScannedNote)
-     : CancelNoteInput :=
+     : UseNoteInput :=
   {
     c := sn.c,
     token := sn.token,
@@ -17,15 +17,15 @@ def spend_note (crypto: Crypto) (m: Memory) (addrbob: ℕ) (kbob: crypto.Private
     amount := sn.amount crypto m,
   }
 
--- A discoverable, uncanceled note with non-zero amount can be spent.
+-- A discoverable, unused note with non-zero amount can be spent.
 theorem spendable_note
     {crypto: Crypto} {rm: ReachableMemory crypto} {sn: ScannedNote}
     (bob: UserPrivKey crypto rm.m)
     (h_note_in_scan: sn ∈ scan_notes_for_recipient₀ (.from rm) bob.addr bob.k)
-    (h_not_canceled: ¬note_canceled crypto rm.m sn.c sn.token sn.i₀ sn.i₁ bob.k)
+    (h_not_used: ¬note_used crypto rm.m sn.c sn.token sn.i₀ sn.i₁ bob.k)
     (h_amount_ne_zero: sn.amount crypto rm.m ≠ 0) :
     let inp := spend_note crypto rm bob.addr bob.k sn
-    (cancel_note crypto inp rm |> process_action crypto rm).success := by
+    (use_note crypto inp rm |> process_action crypto rm).success := by
   have ⟨inp_create, note_imp, h_sn, h_addrbob, h_Kbob⟩ := NoteImplies.from_scan_notes_for_recipient₀ bob.h_k h_note_in_scan
 
   have h_note_id : inp_create.note_id crypto = sn.note_id crypto := by rw [←h_sn]
@@ -36,7 +36,7 @@ theorem spendable_note
 
   have ⟨h_r, h_amount⟩ := note_amount_eq_amount note_imp.in_create_note_actions
 
-  unfold spend_note cancel_note
+  unfold spend_note use_note
   intro inp
 
   simp only [ServerAction.run_all, ServerAction.run, List.foldl_cons, List.foldl_nil, Bool.true_and]
@@ -53,23 +53,23 @@ theorem spendable_note
   · rw [h_note_id] at h_amount
   · exact bob.k.prop
   · exact h_amount_ne_zero
-  · unfold note_canceled at h_not_canceled
-    simp at h_not_canceled
-    exact h_not_canceled
+  · unfold note_used at h_not_used
+    simp at h_not_used
+    exact h_not_used
 
 def spend_notes
     (crypto: Crypto) (m: Memory) (addrbob: ℕ) (kbob: crypto.PrivateKeys)
-    (sns: List ScannedNote) : List CancelNoteInput × Memory :=
+    (sns: List ScannedNote) : List UseNoteInput × Memory :=
   match sns with
   | [] => ⟨[], m⟩
   | sn :: sns =>
     let ⟨inps, m⟩ := spend_notes crypto m addrbob kbob sns
     let inp := spend_note crypto m addrbob kbob sn
-    let m := (cancel_note crypto inp m |> process_action crypto m).1
+    let m := (use_note crypto inp m |> process_action crypto m).1
     ⟨inp :: inps, m⟩
 
 theorem in_spend_notes
-    {crypto: Crypto} {rm: ReachableMemory crypto} {addrbob: ℕ} {kbob: crypto.PrivateKeys} {sns: List ScannedNote} {inp: CancelNoteInput}
+    {crypto: Crypto} {rm: ReachableMemory crypto} {addrbob: ℕ} {kbob: crypto.PrivateKeys} {sns: List ScannedNote} {inp: UseNoteInput}
     (h: inp ∈ (spend_notes crypto rm addrbob kbob sns).1) :
     inp.note_id crypto ∈ sns.map (λ sn ↦ sn.note_id crypto) := by
   induction sns
@@ -85,35 +85,35 @@ theorem in_spend_notes
     case inr h =>
       exact Or.inr (ih h)
 
--- A list of discoverable, uncanceled, non-zero notes can all be spent.
+-- A list of discoverable, unused, non-zero notes can all be spent.
 theorem spendable_notes
     {crypto: Crypto} {rm: ReachableMemory crypto} {sns: List ScannedNote}
     (bob: UserPrivKey crypto rm.m)
     (h_note_in_scan: sns ⊆ scan_notes_for_recipient₀ (.from rm) bob.addr bob.k)
-    (h_not_canceled: ∀ sn ∈ sns, ¬note_canceled crypto rm.m sn.c sn.token sn.i₀ sn.i₁ bob.k)
+    (h_not_used: ∀ sn ∈ sns, ¬note_used crypto rm.m sn.c sn.token sn.i₀ sn.i₁ bob.k)
     (h_amount_ne_zero: ∀ sn ∈ sns, sn.amount crypto rm ≠ 0)
     (h_nodup: sns.Nodup) :
     let res := spend_notes crypto rm bob.addr bob.k sns
     (∃ rm': ReachableMemory crypto,
       rm'.m = res.2 ∧
       scan_notes_for_recipient₀ (.from rm') bob.addr bob.k = scan_notes_for_recipient₀ (.from rm) bob.addr bob.k ∧
-      rm'.actions = res.1.map (λ inp ↦ Action.CancelNote inp) ++ rm.actions ∧
-      (∀ sn ∈ sns, note_canceled crypto rm'.m sn.c sn.token sn.i₀ sn.i₁ bob.k) ∧
+      rm'.actions = res.1.map (λ inp ↦ Action.UseNote inp) ++ rm.actions ∧
+      (∀ sn ∈ sns, note_used crypto rm'.m sn.c sn.token sn.i₀ sn.i₁ bob.k) ∧
       (∀ sn: ScannedNote, sn.amount crypto rm' = sn.amount crypto rm)
     ) := by
   induction sns
   case nil => use rm; simp [spend_notes]
   case cons sn sns ih =>
     simp only [List.cons_subset] at h_note_in_scan
-    simp only [List.mem_cons, forall_eq_or_imp] at h_not_canceled h_amount_ne_zero
+    simp only [List.mem_cons, forall_eq_or_imp] at h_not_used h_amount_ne_zero
     simp only [List.nodup_cons] at h_nodup
-    obtain ⟨rm', h_rm', h_scan, h_actions, h_canceled, h_amounts⟩ :=
-      ih h_note_in_scan.2 h_not_canceled.2 h_amount_ne_zero.2 h_nodup.2
+    obtain ⟨rm', h_rm', h_scan, h_actions, h_used, h_amounts⟩ :=
+      ih h_note_in_scan.2 h_not_used.2 h_amount_ne_zero.2 h_nodup.2
 
     let res₀ := spend_notes crypto rm.m bob.addr bob.k sns
     have h_extends : rm'.extends rm := by simp [ReachableMemory.extends, h_actions]
 
-    have h_success : (run_action crypto (Action.CancelNote (spend_note crypto rm'.m bob.addr bob.k sn)) rm'.m).success := by
+    have h_success : (run_action crypto (Action.UseNote (spend_note crypto rm'.m bob.addr bob.k sn)) rm'.m).success := by
       unfold run_action
       apply spendable_note (bob:=bob.extend h_extends)
       case h_note_in_scan =>
@@ -122,34 +122,34 @@ theorem spendable_notes
       case h_amount_ne_zero =>
         apply note_amount_nz_immutable h_extends sn
         exact h_amount_ne_zero.1
-      case h_not_canceled =>
-        by_contra h_canceled
-        have ⟨addrbob, amount, ⟨cancel_imp⟩⟩ := CancelImplies.from_note_canceled h_canceled
+      case h_not_used =>
+        by_contra h_used
+        have ⟨addrbob, amount, ⟨use_imp⟩⟩ := UseImplies.from_note_used h_used
 
-        have : cancel_note_actions crypto rm' = res₀.1 ++ (cancel_note_actions crypto rm) := by
-          simp only [cancel_note_actions, h_actions, List.filterMap_append,
+        have : used_note_actions crypto rm' = res₀.1 ++ (used_note_actions crypto rm) := by
+          simp only [used_note_actions, h_actions, List.filterMap_append,
             res₀, List.filterMap_map]
           conv in _ ∘ _ => intro x; simp only [Function.comp_apply]
           rw [List.filterMap_some]
 
-        have h_cancel_inp := cancel_imp.in_cancel_note_actions
-        rw [this] at h_cancel_inp
-        simp only [List.mem_append] at h_cancel_inp
+        have h_used_imp := use_imp.in_used_note_actions
+        rw [this] at h_used_imp
+        simp only [List.mem_append] at h_used_imp
 
-        cases h_cancel_inp
-        case inl h_cancel_inp =>
-          dsimp only [res₀] at h_cancel_inp
-          apply in_spend_notes at h_cancel_inp
-          simp only [List.mem_map] at h_cancel_inp
-          have ⟨sn', h_sn', h_note_id'⟩ := h_cancel_inp
+        cases h_used_imp
+        case inl h_used_imp =>
+          dsimp only [res₀] at h_used_imp
+          apply in_spend_notes at h_used_imp
+          simp only [List.mem_map] at h_used_imp
+          have ⟨sn', h_sn', h_note_id'⟩ := h_used_imp
           apply ScannedNote.note_id_eq at h_note_id'
           rw [h_note_id'] at h_sn'
           exact h_nodup.1 h_sn'
-        case inr h_cancel_inp =>
-          have := (CancelImplies.from_cancel_note_actions h_cancel_inp |>.some).h_note_canceled
-          exact h_not_canceled.1 this
+        case inr h_used_imp =>
+          have := (UseImplies.from_used_note_actions h_used_imp |>.some).h_note_used
+          exact h_not_used.1 this
 
-    let rm'' := rm'.add (.CancelNote (spend_note crypto rm' bob.addr bob.k sn)) h_success
+    let rm'' := rm'.add (.UseNote (spend_note crypto rm' bob.addr bob.k sn)) h_success
     use rm''
     refine ⟨?_, h_scan, ?_, ?_, h_amounts⟩
     · simp only [rm'', spend_notes, ReachableMemory.add_m, run_action, h_rm']
@@ -159,16 +159,16 @@ theorem spendable_notes
       cases h_sn'
       case inl h_sn' =>
         unfold rm''
-        rw [note_canceled, ReachableMemory.add_m, run_action]
-        let info := cancel_note_info crypto (spend_note crypto rm'.m bob.addr bob.k sn) rm' h_success
+        rw [note_used, ReachableMemory.add_m, run_action]
+        let info := use_note_info crypto (spend_note crypto rm'.m bob.addr bob.k sn) rm' h_success
         have := info.memory_diff₀
-        unfold spend_note CancelNoteInput.nullifier at this
+        unfold spend_note UseNoteInput.nullifier at this
         rw [h_sn', ←info.h_m', this]
         simp
       case inr h_sn' =>
-        exact note_canceled_monotone_extends (by simp [rm'', ReachableMemory.extends]) (h_canceled sn' h_sn')
+        exact note_used_monotone_extend (by simp [rm'', ReachableMemory.extends]) (h_used sn' h_sn')
 
-def spend_all (crypto: Crypto) (rm: ReachableMemory crypto) (addrbob: ℕ) (kbob: crypto.PrivateKeys) : List CancelNoteInput :=
+def spend_all (crypto: Crypto) (rm: ReachableMemory crypto) (addrbob: ℕ) (kbob: crypto.PrivateKeys) : List UseNoteInput :=
   let sns := scan_notes_for_recipient₀ (.from rm) addrbob kbob
     |>.filter (λ sn ↦ rm.m .Nullifiers [crypto.hash [sn.c, sn.token, sn.i₀, sn.i₁, kbob]] = 0)
   let res := spend_notes crypto rm addrbob kbob sns
@@ -183,21 +183,21 @@ theorem spend_all_props
     ∀ token,
       sum_create_note_amounts crypto rm' bob.addr token
       + sum_deposit_amounts crypto rm' bob.addr token =
-      sum_cancel_note_amounts crypto rm' bob.addr token := by
+      sum_use_note_amounts crypto rm' bob.addr token := by
   let sns := scan_notes_for_recipient₀ (.from rm) bob.addr bob.k
     |>.filter (λ sn ↦ rm.m .Nullifiers [crypto.hash [sn.c, sn.token, sn.i₀, sn.i₁, bob.k]] = 0)
     |>.filter (λ sn ↦ sn.amount crypto rm.m ≠ 0)
-  let cancel_note_inps := spend_all crypto rm bob.addr bob.k
+  let used_note_inps := spend_all crypto rm bob.addr bob.k
 
   have h_note_in_scan : sns ⊆ scan_notes_for_recipient₀ (.from rm) bob.addr bob.k := by
     intro sn h_sn
     rw [List.mem_filter, List.mem_filter] at h_sn
     exact h_sn.1.1
 
-  have h_not_canceled: ∀ sn ∈ sns, ¬note_canceled crypto rm.m sn.c sn.token sn.i₀ sn.i₁ bob.k := by
+  have h_not_used: ∀ sn ∈ sns, ¬note_used crypto rm.m sn.c sn.token sn.i₀ sn.i₁ bob.k := by
     intro sn h_sn
     rw [List.mem_filter, List.mem_filter, decide_eq_true_eq] at h_sn
-    unfold note_canceled
+    unfold note_used
     simp only [ne_eq, Decidable.not_not]
     exact h_sn.1.2
 
@@ -207,8 +207,8 @@ theorem spend_all_props
     simp only [ne_eq]
     exact h_sn.2
 
-  have ⟨rm', _, h_scan_notes_for_recipient, h_actions, h_canceled, h_amounts⟩ :=
-    spendable_notes bob h_note_in_scan h_not_canceled h_amount_ne_zero (by
+  have ⟨rm', _, h_scan_notes_for_recipient, h_actions, h_used, h_amounts⟩ :=
+    spendable_notes bob h_note_in_scan h_not_used h_amount_ne_zero (by
       apply List.Nodup.filter
       apply List.Nodup.filter
       apply scan_notes_for_recipient₀.nodup bob.h_k
@@ -219,7 +219,7 @@ theorem spend_all_props
   use h_extends
 
   intro token
-  simp only [sum_create_note_cancel_note (bob:=bob.extend h_extends), Nat.add_eq_left]
+  simp only [sum_create_note_use_note (bob:=bob.extend h_extends), Nat.add_eq_left]
   apply List.sum_eq_zero
   intro amount h
   have ⟨sn, h⟩ := List.mem_map.1 h
@@ -236,13 +236,13 @@ theorem spend_all_props
   have : rm.m MemoryType.Nullifiers [crypto.hash [sn.c, token, sn.i₀, sn.i₁, bob.k]] = 0 := by
     rw [←h₁] at *
     by_contra h_nullifier_nz
-    exact note_canceled_monotone_extends h_extends h_nullifier_nz this
+    exact note_used_monotone_extend h_extends h_nullifier_nz this
 
   by_contra h_amount_ne_zero
   have h_sn_in_sns : sn ∈ sns := by
     rw [List.mem_filter, List.mem_filter]
     simp [*]
 
-  have := h_canceled sn h_sn_in_sns
+  have := h_used sn h_sn_in_sns
   rw [h₁] at this
   contradiction
