lean/privacy/notes/used_notes.lean
@@ -1,0 +1,202 @@
+import privacy.utils
+import privacy.actions
+import privacy.notes.notes
+import privacy.notes.note_implies
+import privacy.subchannels.subchannels
+
+def note_used (crypto: Crypto) (m: Memory) (c token i₀ i₁ kbob: ℕ) : Prop :=
+  m .Nullifiers [crypto.hash [c, token, i₀, i₁, kbob]] ≠ 0
+
+structure UseImplies₀
+    {crypto: Crypto} (rm: ReachableMemory crypto) (inp: UseNoteInput) where
+  h_action: .UseNote inp ∈ rm.actions
+  (addralice kalice r_create amount_create: ℕ)
+  amount_nz: inp.amount ≠ 0
+  kbob_priv: inp.kbob ∈ crypto.PrivateKeys
+
+abbrev UseImplies₀.inp_create
+    {crypto: Crypto} {rm: ReachableMemory crypto} {inp: UseNoteInput}
+    (self: UseImplies₀ rm inp) : CreateNoteInput :=
+  ⟨self.addralice, self.kalice, inp.addrbob, crypto.priv_to_pub inp.kbob, inp.token, inp.i₀, inp.i₁, self.r_create, self.amount_create⟩
+
+structure UseImplies
+    {crypto: Crypto} (rm: ReachableMemory crypto) (inp: UseNoteInput)
+    extends UseImplies₀ rm inp where
+  h_note_used: note_used crypto rm.m inp.c inp.token inp.i₀ inp.i₁ inp.kbob
+  note_created: NoteImplies rm (toUseImplies₀.inp_create)
+  h_c: toUseImplies₀.inp_create.c crypto = inp.c
+
+theorem UseImplies.h_note_exists
+    {crypto: Crypto} {rm: ReachableMemory crypto} {inp: UseNoteInput}
+    (use_imp: UseImplies rm inp) :
+    rm.m .Notes [inp.note_id crypto, 0] ≠ 0 := by
+  have := use_imp.note_created.h_note_exists
+  unfold note_exists CreateNoteInput.note_id at this
+  simp only [use_imp.h_c] at this
+  exact this
+
+theorem UseImplies.h_kbob₀
+    {crypto: Crypto} {rm: ReachableMemory crypto} {inp: UseNoteInput}
+    (use_imp: UseImplies rm inp) :
+    use_imp.note_created.subchannel.channel.kbob = inp.kbob := by
+  apply crypto.priv_to_pub_inj use_imp.note_created.subchannel.channel.kbob.prop use_imp.kbob_priv
+  rw [use_imp.note_created.h_Kbob]
+
+theorem UseImplies.h_kbob₁
+    {crypto: Crypto} {rm: ReachableMemory crypto} {inp: UseNoteInput}
+    (use_imp: UseImplies rm inp) :
+    rm.m .PublicKeys [inp.addrbob] = crypto.priv_to_pub inp.kbob := by
+  rw [use_imp.note_created.subchannel.channel.bob_registered.public_key, ←h_kbob₀]
+
+theorem UseImplies.next
+    {crypto: Crypto} {rm: ReachableMemory crypto} {inp: UseNoteInput}
+    {action: Action} (success: (run_action crypto action rm.m).success)
+    (use_imp: UseImplies rm inp) :
+    Nonempty (UseImplies (rm.add action success) inp) := by
+  let res : UseImplies₀ (rm.add action success) inp := {
+    h_action := by simp [use_imp.h_action]
+    addralice := use_imp.addralice
+    kalice := use_imp.kalice
+    r_create := use_imp.r_create
+    amount_create := use_imp.amount_create
+    amount_nz := use_imp.amount_nz
+    kbob_priv := use_imp.kbob_priv
+  }
+
+  cases action
+  case UseNote inp' =>
+    let info := use_note_info crypto inp' rm success
+    have : inp.nullifier crypto ≠ inp'.nullifier crypto := by
+      by_contra h
+      have := use_imp.h_note_used
+      rw [note_used, ←UseNoteInput.nullifier, h] at this
+      exact this info.nullifier_didnt_exist
+    exact ⟨{
+      toUseImplies₀ := res,
+      h_note_used := by
+        rw [ReachableMemory.add_m, run_action, ←info.h_m', note_used]
+        rw [info.no_change _ _ (by simp [this])]
+        exact use_imp.h_note_used
+      note_created := Nonempty.some (use_imp.note_created.next success)
+      h_c := use_imp.h_c
+    }⟩
+
+  all_goals exact ⟨{
+    toUseImplies₀ := res,
+    h_note_used := use_imp.h_note_used
+    note_created := Nonempty.some (use_imp.note_created.next success)
+    h_c := use_imp.h_c
+  }⟩
+
+theorem UseImplies.from_action
+    {crypto: Crypto} {rm: ReachableMemory crypto} {inp: UseNoteInput}
+    (h: .UseNote inp ∈ rm.actions) :
+    Nonempty (UseImplies rm inp) := by
+  revert rm
+  apply ReachableMemory.induction
+  case inv₀ => intro h; contradiction
+
+  intro action rm ih success h
+  cases h
+
+  case head =>
+    let info := use_note_info crypto inp rm success
+    have ⟨inp_create, note_imp, h_note_id⟩ := NoteImplies.from_note_exists info.r_ne_zero
+    have ⟨addralice, ⟨subchannel_imp⟩⟩ := SubchannelImplies.from_subchannel_marker_exists info.subchannel_exists
+
+    let res : UseImplies₀ (rm.add (.UseNote inp) success) inp := {
+      h_action := by simp
+      addralice := inp_create.addralice
+      kalice := inp_create.kalice
+      r_create := inp_create.r
+      amount_create := inp_create.amount
+      amount_nz := info.amount_ne_zero
+      kbob_priv := info.kbob_private_key
+    }
+
+    have h_inp_create: inp.c = inp_create.c crypto ∧ inp_create = res.inp_create := by
+      unfold UseImplies₀.inp_create
+      have := crypto.h_hash (Eq.symm h_note_id)
+      injections
+      simp only [*, true_and]
+
+      have := calc subchannel_imp.channel.c
+        _ = inp.c := by simp [subchannel_imp.h_c]
+        _ = inp_create.c crypto := by assumption
+      have ⟨_, _, h_addrbob, h_kbob⟩ := subchannel_imp.channel.same_c this
+      simp only [UseNoteInput.Kbob] at h_addrbob h_kbob
+      rw [←h_addrbob, ←h_kbob]
+
+    exact ⟨{
+      toUseImplies₀ := res,
+      h_note_used := by rw [rm.add_m, run_action, ←info.h_m', note_used, info.memory_diff₀]; simp
+      note_created := h_inp_create.2 ▸ note_imp.next success |>.some
+      h_c := by simp [h_inp_create]
+    }⟩
+
+  case tail h => exact (ih h |>.some).next success
+
+theorem UseImplies.from_note_used
+    {crypto: Crypto} {rm: ReachableMemory crypto} {c token i₀ i₁ kbob: ℕ}
+    (h: note_used crypto rm c token i₀ i₁ kbob) :
+    ∃ addrbob amount, Nonempty (UseImplies rm ⟨c, addrbob, kbob, token, i₀, i₁, amount⟩) := by
+  revert rm
+  apply ReachableMemory.induction
+  case inv₀ => intro h; trivial
+
+  intro action rm ih success h
+  cases action
+  case UseNote inp =>
+    let info := use_note_info crypto inp rm success
+    have ⟨kalice, ⟨subchannel_imp⟩⟩ := SubchannelImplies.from_subchannel_marker_exists info.subchannel_exists
+    by_cases h_is_same : crypto.hash [c, token, i₀, i₁, kbob] = inp.nullifier crypto
+    case pos =>
+      use inp.addrbob, inp.amount
+      have := crypto.h_hash h_is_same
+      repeat injection this with _ this
+      apply UseImplies.from_action
+      simp [*]
+    case neg =>
+      rw [note_used, ReachableMemory.add_m, run_action, ←info.h_m'] at h
+      rw [info.no_change _ _ (by simp [h_is_same])] at h
+      have ⟨addrbob, amount, ⟨use_imp⟩⟩ := ih h
+      exact ⟨addrbob, amount, use_imp.next success⟩
+
+  all_goals
+    have ⟨addrbob, amount, ⟨use_imp⟩⟩ := ih h
+    exact ⟨addrbob, amount, use_imp.next success⟩
+
+def used_note_actions (crypto: Crypto) (rm: ReachableMemory crypto) : List UseNoteInput :=
+  rm.actions.filterMap filter_UseNote
+
+theorem used_note_actions_add
+    {crypto: Crypto} {rm: ReachableMemory crypto} {inp: UseNoteInput}
+    (success: (run_action crypto (.UseNote inp) rm.m).success) :
+    (used_note_actions crypto (rm.add (.UseNote inp) success)) =
+    inp :: used_note_actions crypto rm := by
+  simp [used_note_actions]
+
+theorem UseImplies.in_used_note_actions
+    {crypto: Crypto} {rm: ReachableMemory crypto} {inp: UseNoteInput}
+    (note_imp: UseImplies rm inp) :
+    inp ∈ used_note_actions crypto rm := by
+  simp [used_note_actions]
+  use .UseNote inp
+  simp [note_imp.h_action]
+
+theorem UseImplies.from_used_note_actions
+    {crypto: Crypto} {rm: ReachableMemory crypto} {inp: UseNoteInput}
+    (h: inp ∈ used_note_actions crypto rm) :
+    Nonempty (UseImplies rm inp) := by
+  simp only [used_note_actions, List.mem_filterMap, filter_UseNote_some, exists_eq_right] at h
+  exact UseImplies.from_action h
+
+theorem note_used_monotone_extend
+    {crypto: Crypto} {rm rm': ReachableMemory crypto}
+    (h_extends: rm'.extends rm)
+    (h: note_used crypto rm c token i₀ i₁ kbob) :
+    note_used crypto rm' c token i₀ i₁ kbob := by
+  have ⟨addrbob, amount, ⟨use_imp⟩⟩ := UseImplies.from_note_used h
+  have ⟨ℓ, h_extends⟩ := h_extends
+  have := h_extends ▸ (List.mem_append (s:=ℓ)).2 (Or.inr use_imp.h_action)
+  exact (UseImplies.from_action this |>.some).h_note_used
