lean/privacy/tracing/incoming_notes.lean
@@ -1,7 +1,7 @@
 import privacy.actions
 import privacy.amounts
 import privacy.compliance.all_notes
-import privacy.notes.canceled_notes
+import privacy.notes.used_notes
 import privacy.registration.discoverable
 import privacy.transactions.transactions
 import privacy.tracing.utils
@@ -17,16 +17,16 @@ theorem incoming_notes
     ) = (
       stxs.txs
       |>.filter (λ tx ↦ tx.owner = bob.addr)
-      |>.map (λ tx ↦ tx.sum_cancel_note_amounts token)
+      |>.map (λ tx ↦ tx.sum_use_note_amounts token)
       |>.sum
     ) := by
-  rw [←sum_of_canceled_notes_to_scanned_notes bob token]
+  rw [←sum_of_used_notes_to_scanned_notes bob token]
   rw [←filtered_note_actions_to_tx_actions]
-  unfold sum_cancel_note_amounts cancel_note_actions ActionFunc.cancel ActionFuncRes.from_cancel
+  unfold sum_use_note_amounts used_note_actions ActionFunc.use ActionFuncRes.from_use
   simp only [List.filter_filterMap, List.map_filterMap]
   apply congrArg
   apply List.filterMap_congr
   intro action h_action
-  cases h_some: filter_CancelNote action
+  cases h_some: filter_UseNote action
   case none => simp
   case some inp => simp [Option.filter_some]
